

DATE: 10/06/2025

Anecto, Mary Kate F.

$$f(x) = x^3 - 4x + 1, \text{ (2) 4 iterations}$$

$$\begin{aligned} \textcircled{1} \quad f(x) &= x^3 - 4x + 1 & f'(x) &= 3x^{3-1} - 4 & x_{n+1} &= 2 - \left( \frac{1}{8} \right) = \frac{16-1}{8} = \frac{15}{8} \\ & & &= 3x^2 - 4 & & \\ &= 2^3 - 4(2) + 1 & &= 3(2)^2 - 4 & &= \boxed{1.875} \\ &= 8 - 8 + 1 & &= 3(4) - 4 & &1.875 - 1 = 0.875 \\ &= 0 + 1 & &= 12 - 4 & & \\ &= 1 & &= 8 & & \end{aligned}$$

$$\begin{aligned} \textcircled{2} \quad f(1.875) &= (1.875)^3 - 4(1.875) + 1 & f'(1.875) &= 3(1.875)^2 - 4 \\ &= 6.592 - 7.5 + 1 & &= 3(3.516) - 4 \\ &= -0.908 + 1 & &= 10.548 - 4 \\ &= 0.092 & &= 6.548 & &1.861 - 1 = 0.861 \\ x_{n+1} &= 1.875 - \left( \frac{0.092}{6.548} \right) = 1.875 - 0.014 = \boxed{1.861} \end{aligned}$$

$$\begin{aligned} \textcircled{3} \quad f(1.861) &= (1.861)^3 - 4(1.861) + 1 & f'(1.861) &= 3(1.861)^2 - 4 \\ &= 6.445 - 7.444 + 1 & &= 3(3.463) - 4 \\ &= -0.999 + 1 & &= 10.389 - 4 \\ &= 0.001 & &= 6.389 \\ x_{n+1} &= 1.861 - \left( \frac{0.001}{6.389} \right) = 1.861 - 0.000 = \boxed{1.861} & &1.861 - 1 = 0.861 \end{aligned}$$

$$\begin{aligned} \textcircled{4} \quad f(1.861) &= (1.861)^3 - 4(1.861) + 1 & f'(1.861) &= 3(1.861)^2 - 4 \\ &= 6.445 - 7.444 + 1 & &= 3(3.463) - 4 \\ &= -0.999 + 1 & &= 10.389 - 4 \\ &= 0.001 & &= 6.389 & &1.861 - 1 = 0.861 \\ x_{n+1} &= 1.861 - \left( \frac{0.001}{6.389} \right) = 1.861 - 0.000 = \boxed{1.861} \end{aligned}$$

$$f(x) = x^3 - 2x^2 + 3, \text{ (1) 4 iterations}$$

$$\begin{aligned} \textcircled{1} \quad f(x) &= x^3 - 2x^2 + 3 & f'(x) &= 3x^{3-1} - 2(2)x^{2-1} \\ & & &= 3x^2 - 4x & x_{n+1} &= 1 - \left( \frac{2}{-1} \right) = 1 + 2 = \boxed{3} \\ f(1) &= 1^3 - 2(1)^2 + 3 & f'(1) &= 3(1)^2 - 4(1) & & \\ &= 1 - 2(1) + 3 & &= 3 - 4 & &3 - 1 = 2 \\ &= 1 - 2 + 3 & &= -1 & & \\ &= -1 + 3 & & & & \\ &= 2 & & & & \end{aligned}$$

$$\begin{aligned} \textcircled{2} \quad f(3) &= 3^3 - 2(3)^2 + 3 & f'(3) &= 3(3)^2 - 4(3) & x_{n+1} &= 3 - \left( \frac{12^{+3}}{15} \right) = 3 - \frac{4}{5} \\ &= 27 - 2(9) + 3 & &= 3(9) - 12 & & \\ &= 27 - 18 + 3 & &= 27 - 12 & &= \frac{15 - 4}{5} = \frac{11}{5} \\ &= 9 + 3 & &= 15 & & \\ &= 12 & & & &= \boxed{2.2} \end{aligned}$$

$$\begin{aligned} \textcircled{3} \quad f(2.2) &= (2.2)^3 - 2(2.2)^2 + 3 & f'(2.2) &= 3(2.2)^2 - 4(2.2) \\ &= 10.648 - 2(4.840) + 3 & &= 3(4.84) - 8.8 \\ &= 10.648 - 9.680 + 3 & &= 14.52 - 8.8 \\ &= 0.968 + 3 & &= 5.720 \\ &= 3.968 & & & &1.506 - 1 = 0.506 \end{aligned}$$

$$x_{n+1} = 2.2 - \left( \frac{3.968}{5.720} \right) = 2.2 - 0.694 = \boxed{1.506}$$

$$\begin{aligned} \textcircled{4} \quad f(1.506) &= (1.506)^3 - 2(1.506)^2 + 3 & f'(1.506) &= 3(1.506)^2 - 4(1.506) \\ &= 3.416 - 2(2.268) + 3 & &= 3(2.268) - 6.024 \\ &= 3.416 - 4.536 + 3 & &= 6.804 - 6.024 \\ &= -1.12 + 3 & &= 0.780 \\ &= 1.88 & & & &1 - (-0.904) = 1.904 \end{aligned}$$

$$x_{n+1} = 1.506 - \left( \frac{1.88}{0.780} \right) = 1.506 - 2.410 = \boxed{-0.904}$$

$$f(x) = x^2 - 2x - 5 \quad \textcircled{2} \quad 3 \text{ Iterations}$$

$$\begin{aligned} \textcircled{1} \quad f(x) &= x^2 - 2x - 5 & f'(x) &= 2x^{2-1} - 2 & x_{n+1} &= 2 - \left( \frac{-5}{2} \right) \\ f(2) &= 2^2 - 2(2) - 5 & &= 2x - 2 & & \\ &= 4 - 4 - 5 & f'(2) &= 2(2) - 2 & &= \frac{4 + 5}{2} = \frac{9}{2} = \boxed{4.5} \\ &= -5 & &= 4 - 2 & & \\ & & &= 2 & & \end{aligned}$$

$$\begin{aligned} \textcircled{2} \quad f(4.5) &= (4.5)^2 - 2(4.5) - 5 & f'(4.5) &= 2(4.5) - 2 \\ &= 20.25 - 9 - 5 & &= 9 - 2 \\ &= 11.25 - 5 & &= 7 \\ &= 6.25 & & & &3.607 - 2 = 1.607 \end{aligned}$$

$$x_{n+1} = 4.5 - \left( \frac{6.25}{7} \right) = 4.5 - 0.893 = \boxed{3.607}$$



2/2

DATE: 10/06/2025

Aneito, Mary Kate F.

$$\begin{aligned}\textcircled{3} f(3.607) &= (3.607)^2 - 2(3.607) - 5 \\ &= 13.010 - 7.214 - 5 \\ &= 5.796 - 5 \\ &= 0.796\end{aligned}$$

$$\begin{aligned}f'(3.607) &= 2(3.607) - 2 \\ &= 7.214 - 2 \\ &= 5.214\end{aligned}$$

$$3.454 - 2 = 1.454$$

$$X_{n+1} = 3.607 - \left( \frac{0.796}{5.214} \right) = 3.607 - 0.153 = \boxed{3.454}$$